Base64: add base64UrlLookup

Clap/Base64Len.lean
@@ -12,6 +12,48 @@ def base64UrlDecodedLength (w : ℕ) (m : F p) : Option (F p) := do
   let bits ← num2bits (w + 2) three      -- decompose 3m, proves < 2^(w+2)
   return bits2num (bits.drop 2)          -- drop 2 LSBs = floor(3m/4)\
 
+def base64UrlLookup (i : F p) : Option (F p) := do
+  -- check if i ∈ ['A', 'Z']
+  let ge_A ← F.greaterEqThan 8 i 65
+  let le_Z ← F.lessEqThan 8 i 90
+  let range_AZ := FB.and ge_A le_Z
+  let sum_AZ := convert range_AZ * (i - 65)
+
+  -- check if i ∈ ['a', 'z']
+  let ge_a ← F.greaterEqThan 8 i 97
+  let le_z ← F.lessEqThan 8 i 122
+  let range_az := FB.and ge_a le_z
+  let sum_az := sum_AZ + convert range_az * (i - 71)
+
+  -- check if i ∈ ['0', '9']
+  let ge_a ← F.greaterEqThan 8 i 48
+  let le_z ← F.lessEqThan 8 i 57
+  let range_09 := FB.and ge_a le_z
+  let sum_09 := sum_az + convert range_09 * (i + 4)
+
+  -- check if i is '-'
+  let eq_minus := isZero (i - 45)
+  let sum_minus := sum_09 + convert eq_minus * 62;
+
+  -- check if i is '_'
+  let eq_underscore := isZero (i - 95)
+  let sum_underscore := sum_minus + convert eq_underscore * 63;
+
+  -- check if i is '='
+  let eq_eqsign := isZero (i - 61)
+
+  -- check if i is zero
+  let zero_padding := isZero i
+
+  -- exactly one case has to be true
+  [range_AZ, range_az, range_09, eq_minus, eq_underscore, eq_eqsign, zero_padding]
+    |> List.map convert
+    |> List.sum
+    |> (· - 1)
+    |> eq0
+
+  pure sum_underscore
+
 end Base64Len
 
 namespace TestBase64Len
@@ -20,6 +62,18 @@ open Clap.Lang Core ZMod
 open Base64Len
 
 abbrev p := Primes.goldilocks
+
+example : base64UrlLookup (p := p) 'A'.toNat == some 0 := by native_decide
+example : base64UrlLookup (p := p) 'Z'.toNat == some 25 := by native_decide
+example : base64UrlLookup (p := p) 'a'.toNat == some 26 := by native_decide
+example : base64UrlLookup (p := p) 'z'.toNat == some 51 := by native_decide
+example : base64UrlLookup (p := p) '0'.toNat == some 52 := by native_decide
+example : base64UrlLookup (p := p) '9'.toNat == some 61 := by native_decide
+example : base64UrlLookup (p := p) '-'.toNat == some 62 := by native_decide
+example : base64UrlLookup (p := p) '_'.toNat == some 63 := by native_decide
+example : base64UrlLookup (p := p) '='.toNat == some 0 := by native_decide
+example : base64UrlLookup (p := p) 0 == some 0 := by native_decide
+example : base64UrlLookup (p := p) 64 == none := by native_decide
 
 example : base64UrlDecodedLength (p := p) 8 0  = some 0  := by native_decide
 example : base64UrlDecodedLength (p := p) 8 2  = some ((3 * 2 / 4) : Nat)  := by native_decide
